wand lemmas

split/strong.v
@@ -19,8 +19,6 @@ Import Ctypes LiftNotation.
 Local Open Scope logic.
 Require Import split.vst_ext.
 
-
-
 Definition obox (Delta: tycontext) (i: ident) (P: environ -> mpred): environ -> mpred :=
   ALL v: _,
     match ((temp_types Delta) ! i) with
@@ -33,7 +31,6 @@ Definition oboxopt Delta ret P :=
   | Some id => obox Delta id P
   | _ => P
   end.
-
 
 
 Inductive semax_aux {CS: compspecs} {Espec: OracleKind} (Delta: tycontext): (environ -> mpred) -> Clight.statement -> ret_assert -> Prop :=
@@ -55,25 +52,20 @@ Inductive semax_aux {CS: compspecs} {Espec: OracleKind} (Delta: tycontext): (env
      @semax_aux CS Espec Delta  Q body (loop1_ret_assert Q' R) ->
      @semax_aux CS Espec Delta Q' incr (loop2_ret_assert Q R) ->
      @semax_aux CS Espec Delta Q (Clight.Sloop body incr) R
-| semax_aux_call_backward: forall ret a bl R,
-     @semax_aux CS Espec Delta
-         (EX argsig: _, EX retsig: _, EX cc: _,
-          EX A: _, EX P: _, EX Q: _, EX NEP: _, EX NEQ: _, EX ts: _, EX x: _,
-         !! (Cop.classify_fun (typeof a) =
-             Cop.fun_case_f (type_of_params argsig) retsig cc /\
-             (retsig = Tvoid -> ret = None) /\
-             tc_fn_return Delta ret retsig) &&
-          (((tc_expr Delta a) && (tc_exprlist Delta (snd (split argsig)) bl)))  &&
-         `(func_ptr (mk_funspec  (argsig,retsig) cc A P Q NEP NEQ)) (eval_expr a) &&
-          |>((`(P ts x: environ -> mpred) (make_args' (argsig,retsig) (eval_exprlist (snd (split argsig)) bl))) * oboxopt Delta ret (maybe_retval (Q ts x) retsig ret -* R)))
-         (Clight.Scall ret a bl)
-         (normal_ret_assert R)
 | semax_aux_return: forall (R: ret_assert) ret ,
       @semax_aux CS Espec Delta
                 ( (tc_expropt Delta ret (ret_type Delta)) &&
                 `(RA_return R : option val -> environ -> mpred) (cast_expropt ret (ret_type Delta)) (@id environ))
                 (Clight.Sreturn ret)
                 R
+| semax_aux_skip: forall P, @semax_aux CS Espec Delta P Clight.Sskip (normal_ret_assert P)
+| semax_aux_assign: forall (P: environ->mpred) e1 e2,
+    @semax_aux CS Espec Delta
+    (EX sh: share, !! writable_share sh &&
+      (|> ( (tc_lvalue Delta e1) &&  (tc_expr Delta (Ecast e2 (typeof e1)))  &&
+      ((`(mapsto_ sh (typeof e1)) (eval_lvalue e1)) * (`(mapsto sh (typeof e1)) (eval_lvalue e1) (`force_val (`(sem_cast (typeof e2) (typeof e1)) (eval_expr e2))) -* P)))))
+          (Clight.Sassign e1 e2)
+          (normal_ret_assert P)
 | semax_aux_set_ptr_compare_load_cast_load_backward: forall (P: environ->mpred) id e,
     @semax_aux CS Espec Delta
        ((|> ( (tc_expr Delta e) &&
@@ -111,14 +103,6 @@ Inductive semax_aux {CS: compspecs} {Espec: OracleKind} (Delta: tycontext): (env
               (`(mapsto sh (typeof e1)) (eval_lvalue e1) (`v2) * TT) &&
               subst id (`(force_val (sem_cast (typeof e1) t1 v2))) P)))
         (Clight.Sset id e) (normal_ret_assert P)
-| semax_aux_store_backward: forall e1 e2 P,
-   @semax_aux CS Espec Delta
-          (EX sh: share, !! writable_share sh && |> ( (tc_lvalue Delta e1) &&  (tc_expr Delta (Ecast e2 (typeof e1)))  &&
-             ((`(mapsto_ sh (typeof e1)) (eval_lvalue e1)) * (`(mapsto sh (typeof e1)) (eval_lvalue e1) (`force_val (`(sem_cast (typeof e2) (typeof e1)) (eval_expr e2))) -* P))))
-          (Clight.Sassign e1 e2)
-          (normal_ret_assert P)
-| semax_aux_skip: forall P, @semax_aux CS Espec Delta P Clight.Sskip (normal_ret_assert P)
-| semax_aux_builtin: forall P opt ext tl el, @semax_aux CS Espec Delta FF (Clight.Sbuiltin opt ext tl el) P
 | semax_aux_conseq: forall P' (R': ret_assert) P c (R: ret_assert) ,
     (local (tc_environ Delta) && (allp_fun_id Delta && P) |-- P') ->
     local (tc_environ Delta) && (allp_fun_id Delta && RA_normal R') |-- RA_normal R ->
@@ -126,7 +110,6 @@ Inductive semax_aux {CS: compspecs} {Espec: OracleKind} (Delta: tycontext): (env
     local (tc_environ Delta) && (allp_fun_id Delta && RA_continue R') |-- RA_continue R ->
     (forall vl, local (tc_environ Delta) && (allp_fun_id Delta && RA_return R' vl) |-- RA_return R vl) ->
     @semax_aux CS Espec Delta P' c R' -> @semax_aux CS Espec Delta P c R.
-
 
 Inductive semax {CS: compspecs} {Espec: OracleKind} (Delta: tycontext): (environ -> mpred) -> Clight.statement -> ret_assert -> Prop :=
 (* | semax_aux_intro :
@@ -190,13 +173,31 @@ Proof.
     solve_andp.
 Qed.
 
+Ltac unfold_der := unfold overridePost, RA_normal, RA_break, RA_continue, RA_return in *.
+
 Lemma semax_aux_seq_inv: forall CS Espec (Delta : tycontext) (P : environ -> mpred) 
       (R : ret_assert) (h t : Clight.statement),
     @semax_aux CS Espec Delta P (Clight.Ssequence h  t)%C R ->
     exists Q : environ -> mpred,
       @semax_aux CS Espec Delta P h (overridePost Q R) /\
       @semax_aux CS Espec Delta Q t R.
-Admitted.
+Proof.
+  intros.
+  remember (Clight.Ssequence h  t)%C as c.
+  induction H;inversion Heqc.
+  + subst. exists Q. auto.
+  + specialize (IHsemax_aux H5).
+    destruct IHsemax_aux as [Q [? ?]].
+    exists Q. split.
+    - eapply semax_aux_conseq;[..|apply H6];auto;
+      destruct R as [Rn Rb Rc Rr];
+      destruct R' as [Rn' Rb' Rc' Rr']; unfold_der;auto.
+      solve_andp.
+    - eapply semax_aux_conseq;[..|apply H7];auto;
+      destruct R as [Rn Rb Rc Rr];
+      destruct R' as [Rn' Rb' Rc' Rr']; unfold_der;auto.
+      solve_andp.
+Qed.
 
 
 Lemma semax_aux_seq_inv': forall CS Espec (Delta : tycontext) (P : environ -> mpred) 
@@ -206,7 +207,391 @@ Lemma semax_aux_seq_inv': forall CS Espec (Delta : tycontext) (P : environ -> mp
          (overridePost
             (EX Q : environ -> mpred,
              !! semax_aux Delta Q t R && Q)%assert R).
+Proof.
+  intros.
+  remember (Clight.Ssequence h  t)%C as c.
+  induction H;inversion Heqc.
+  + subst. eapply semax_aux_conseq;[..|apply H];auto;
+    destruct R as [Rn Rb Rc Rr]; unfold_der;auto;intros; try solve_andp.
+    Exists Q. apply andp_right;try solve_andp. apply prop_right.
+    auto.
+  + specialize (IHsemax_aux H5).
+    eapply semax_aux_conseq;[..|apply IHsemax_aux];auto;
+      destruct R as [Rn Rb Rc Rr];
+      destruct R' as [Rn' Rb' Rc' Rr']; unfold_der;auto.
+    Intros Q. Exists Q.
+    apply andp_right;try solve_andp. apply prop_right.
+    eapply semax_aux_conseq;[..|apply H6];auto;
+    unfold_der;auto.
+    solve_andp.
+Qed.
+
+Lemma semax_aux_assign_inv: forall {CS: compspecs} {Espec: OracleKind} 
+Delta e1 e2 P Q,
+@semax_aux CS Espec Delta P (Clight.Sassign e1 e2) Q ->
+local (tc_environ Delta) && (allp_fun_id Delta && P) |-- 
+(EX sh: share, !! writable_share sh 
+    && |> ( (tc_lvalue Delta e1) &&  (tc_expr Delta (Ecast e2 (typeof e1)))  &&
+           ((`(mapsto_ sh (typeof e1)) (eval_lvalue e1)) * (`(mapsto sh (typeof e1)) (eval_lvalue e1) (`force_val (`(sem_cast (typeof e2) (typeof e1)) (eval_expr e2))) -* RA_normal Q)))).
+Proof.
+intros.
+remember (Clight.Sassign e1 e2) as c eqn:?H.
+induction H;try solve [inv H0].
++ inv H0. reduce2derives. Intros sh. Exists sh.
+  apply andp_right. { apply prop_right. auto. }
+  unfold normal_ret_assert. unfold RA_normal.
+  apply later_derives; auto.
++ subst c. specialize (IHsemax_aux eq_refl).
+  eapply derives_trans with (Q:= (andp (local (tc_environ Delta)) (andp (allp_fun_id Delta) P'))).
+  { repeat (apply andp_right;try solve_andp). auto. }
+  eapply derives_trans.
+  { apply andp_right with (P0:=local (tc_environ Delta)). solve_andp.
+    apply andp_right with (P0:=
+     allp_fun_id Delta). solve_andp. apply derives_refl. }
+  eapply derives_trans.
+  { apply andp_right. apply andp_left1. apply derives_refl.
+    apply andp_right. apply andp_left2. apply andp_left1. apply derives_refl.
+    apply andp_left2. apply andp_left2.
+    apply IHsemax_aux. }
+  reduceR. Intros sh. Exists sh.
+  apply andp_right.
+  { apply prop_right. auto. }
+  apply later_ENTAILL.
+  apply andp_ENTAILL; [reduceLL; apply ENTAIL_refl |].
+  apply sepcon_ENTAILL; [reduceLL; apply ENTAIL_refl |].
+  apply wand_ENTAILL; [reduceLL; apply ENTAIL_refl |].
+  auto.
+Qed.
+
+
+Lemma semax_aux_set_inv: forall {CS: compspecs} {Espec: OracleKind} Delta P R id e,
+  @semax_aux CS Espec Delta P (Clight.Sset id e) R ->
+  local (tc_environ Delta) && (allp_fun_id Delta && P) |-- 
+    ( (|> ( (tc_expr Delta e) &&
+             (tc_temp_id id (typeof e) Delta e) &&
+             subst id (eval_expr e) (RA_normal R))) ||
+      (EX cmp: Cop.binary_operation, EX e1: expr, EX e2: expr,
+         EX ty: type, EX sh1: share, EX sh2: share,
+          !! (e = Ebinop cmp e1 e2 ty /\
+              sepalg.nonidentity sh1 /\ sepalg.nonidentity sh2 /\
+              is_comparison cmp = true /\
+              eqb_type (typeof e1) int_or_ptr_type = false /\
+              eqb_type (typeof e2) int_or_ptr_type = false /\
+              typecheck_tid_ptr_compare Delta id = true) &&
+            ( |> ( (tc_expr Delta e1) &&
+              (tc_expr Delta e2)  &&
+          local (`(blocks_match cmp) (eval_expr e1) (eval_expr e2)) &&
+          (`(mapsto_ sh1 (typeof e1)) (eval_expr e1) * TT) &&
+          (`(mapsto_ sh2 (typeof e2)) (eval_expr e2) * TT) &&
+          subst id (eval_expr (Ebinop cmp e1 e2 ty)) (RA_normal R)))) ||
+      (EX sh: share, EX t2: type, EX v2: val,
+              !! (typeof_temp Delta id = Some t2 /\
+                  is_neutral_cast (typeof e) t2 = true /\
+                  readable_share sh) &&
+         |> ( (tc_lvalue Delta e) &&
+              local (`(tc_val (typeof e) v2)) &&
+              (`(mapsto sh (typeof e)) (eval_lvalue e) (`v2) * TT) &&
+              subst id (`v2) (RA_normal R))) ||
+      (EX sh: share, EX e1: expr, EX t1: type, EX v2: val,
+              !! (e = Ecast e1 t1 /\
+                  typeof_temp Delta id = Some t1 /\
+                  cast_pointer_to_bool (typeof e1) t1 = false /\
+                  readable_share sh) &&
+         |> ( (tc_lvalue Delta e1) &&
+              local (`(tc_val t1) (`(eval_cast (typeof e1) t1 v2))) &&
+              (`(mapsto sh (typeof e1)) (eval_lvalue e1) (`v2) * TT) &&
+              subst id (`(force_val (sem_cast (typeof e1) t1 v2))) (RA_normal R)))).
+Proof.
+  intros.
+  remember (Clight.Sset id e) as c eqn:?H.
+  induction H; try solve [inv H0].
+  + inv H0.
+    reduce2derives.
+    apply orp_derives; [apply orp_derives; [apply orp_derives |] |].
+    - apply later_derives.
+      apply andp_derives; auto.
+      apply subst_derives. unfold normal_ret_assert.
+      unfold RA_normal. auto.
+    - apply exp_derives; intros cmp.
+      apply exp_derives; intros e1.
+      apply exp_derives; intros e2.
+      apply exp_derives; intros ty.
+      apply exp_derives; intros sh1.
+      apply exp_derives; intros sh2.
+      apply andp_derives; auto.
+      apply later_derives; auto.
+      apply andp_derives; auto.
+      apply subst_derives. unfold normal_ret_assert.
+      unfold RA_normal. auto.
+    - apply exp_derives; intros sh.
+      apply exp_derives; intros t2.
+      apply exp_derives; intros v2.
+      apply andp_derives; auto.
+      apply later_derives.
+      apply andp_derives; auto.
+      apply subst_derives. unfold normal_ret_assert.
+      unfold RA_normal. auto.
+    - apply exp_derives; intros sh.
+      apply exp_derives; intros e1.
+      apply exp_derives; intros t1.
+      apply exp_derives; intros v2.
+      apply andp_derives; auto.
+      apply later_derives.
+      apply andp_derives; auto.
+      apply subst_derives. unfold normal_ret_assert.
+      unfold RA_normal. auto.
+  + subst c.
+    rename P into Pre, R into Post. specialize (IHsemax_aux eq_refl).
+    eapply derives_trans with (Q:= (andp (local (tc_environ Delta)) (andp (allp_fun_id Delta) P'))).
+    { repeat (apply andp_right;try solve_andp). auto. }
+    eapply derives_trans.
+    { apply andp_right with (P:=local (tc_environ Delta)). solve_andp.
+      apply andp_right with (P:=
+      allp_fun_id Delta). solve_andp. apply derives_refl. }
+    eapply derives_trans.
+    { apply andp_right. apply andp_left1. apply derives_refl.
+      apply andp_right. apply andp_left2. apply andp_left1. apply derives_refl.
+      apply andp_left2. apply andp_left2.
+      apply IHsemax_aux. }
+      reduceR.
+    apply orp_ENTAILL; [apply orp_ENTAILL; [apply orp_ENTAILL |] |].
+    - apply later_ENTAILL.
+      unfold tc_temp_id, typecheck_temp_id.
+      destruct ((temp_types Delta) ! id) eqn:?H; [| normalize].
+      eapply andp_subst_ENTAILL; [eauto | | reduceLL; apply ENTAIL_refl |].
+      * destruct (is_neutral_cast (implicit_deref (typeof e)) t) eqn:?H; [| normalize].
+        intro rho; unfold_lift; unfold local, lift1; simpl.
+        normalize.
+        apply andp_left2, andp_left1.
+        eapply derives_trans; [apply typecheck_expr_sound; auto |].
+        normalize.
+        intros _.
+        eapply expr2.neutral_cast_subsumption'; eauto.
+      * auto.
+    - apply exp_ENTAILL; intro cmp.
+      apply exp_ENTAILL; intro e1.
+      apply exp_ENTAILL; intro e2.
+      apply exp_ENTAILL; intro ty.
+      apply exp_ENTAILL; intro sh1.
+      apply exp_ENTAILL; intro sh2.
+      normalize. apply andp_right.
+      { apply prop_right. repeat split;auto. }
+      apply later_ENTAILL.
+      unfold typecheck_tid_ptr_compare in H10.
+      destruct ((temp_types Delta) ! id) eqn:?H; [| inv H10].
+      eapply andp_subst_ENTAILL; [eauto | | reduceLL; apply ENTAIL_refl |].
+      * unfold_lift; unfold local, lift1; intro rho.
+        simpl. normalize.
+        apply andp_left2, andp_left1. apply andp_left1.
+        eapply derives_trans; [apply andp_derives; apply typecheck_expr_sound; auto |].
+        normalize.
+        unfold_lift.
+        replace (sem_binary_operation' cmp) with (sem_cmp (expr.op_to_cmp cmp)); [| destruct cmp; inv H7; auto].
+        apply binop_lemmas2.tc_val'_sem_cmp; auto.
+      * auto.
+    - apply exp_ENTAILL; intro sh.
+      apply exp_ENTAILL; intro t2.
+      apply exp_ENTAILL; intro v2.
+      normalize.
+      (* destruct H0 as [? [? ?]].
+      apply later_ENTAILL.
+      unfold typeof_temp in H0.
+      destruct ((temp_types Delta) ! id) eqn:?H; inv H0.
+      eapply andp_subst_ENTAILL; [eauto | | reduceLL; apply ENTAIL_refl |].
+      * reduceL.
+        apply andp_left1.
+        apply andp_left2.
+        unfold_lift; unfold local, lift1; intro rho; simpl; normalize.
+        intros _; eapply expr2.neutral_cast_subsumption; eauto.
+      * apply derives_full_bupd0_left.
+        auto.
+    - apply exp_ENTAILL; intro sh.
+      apply exp_ENTAILL; intro e1.
+      apply exp_ENTAILL; intro t1.
+      apply exp_ENTAILL; intro t2.
+      normalize.
+      destruct H0 as [He [? [? ?]]].
+      apply later_ENTAILL.
+      unfold typeof_temp in H0.
+      destruct ((temp_types Delta) ! id) eqn:?H; inv H0.
+      eapply andp_subst_ENTAILL; [eauto | | reduceLL; apply ENTAIL_refl |].
+      * reduceL.
+        apply andp_left1.
+        apply andp_left2.
+        unfold_lift; unfold local, lift1; intro rho; simpl; normalize.
+        intros _; auto.
+      * apply derives_full_bupd0_left.
+        auto.
+Qed. *)
 Admitted.
+
+(* Lemma wsh_relation: forall sh1 sh2 t e v Q1 Q2 ,
+  writable_share sh1 -> writable_share sh2 ->
+  (((mapsto sh1 t e v) -* Q1) && ((mapsto sh2 t e v) -* Q2) |--
+  EX sh:share, !! (writable_share sh) &&  ((mapsto sh t e v) -* (Q1 && Q2))).
+Proof.
+  intros.
+  hnf in H. destruct H .
+  hnf in H. hnf in H1.
+  Exists Tsh. apply andp_right.
+  2:{ apply wand_frame_intro'.
+      eapply derives_trans.
+      { apply distrib_sepcon_andp. }
+      apply andp_right.
+      - apply andp_left1.
+      Search mapsto.
+        unfold mapsto at 1. Print access_mode.
+        Print By_value.
+
+
+        pose proof join_comp_Tsh.
+        Search mapsto sepcon.
+        Search sepcon derives.
+      Search Tsh sepalg.join.
+  Search sepcon andp.
+  Search wand derives. }
+  Search sepalg.identity. Search sepcon andp.
+  unfold sepalg.identity in H.
+  
+  unfold writable_share.
+  Search share. *)
+
+
+(* Lemma semax_aux_assign_inv: forall {CS: compspecs} {Espec: OracleKind} 
+  Delta e1 e2 P Q,
+@semax_aux CS Espec Delta P (Clight.Sassign e1 e2) Q ->
+  local (tc_environ Delta) && (allp_fun_id Delta && P) |-- 
+  (EX sh: share, !! writable_share sh 
+      && |> ( (tc_lvalue Delta e1) &&  (tc_expr Delta (Ecast e2 (typeof e1)))  &&
+             ((`(mapsto_ sh (typeof e1)) (eval_lvalue e1)) * (`(mapsto sh (typeof e1)) (eval_lvalue e1) (`force_val (`(sem_cast (typeof e2) (typeof e1)) (eval_expr e2))) -* RA_normal Q)))).
+Proof.
+  intros.
+  remember (Clight.Sassign e1 e2) as c eqn:?H.
+  induction H;try solve [inv H0].
+  + inv H0. reduce2derives. Exists sh.
+    apply andp_right. { apply prop_right. auto. }
+    unfold normal_ret_assert. unfold RA_normal. *)
+
+(*
+
+Lemma semax_aux_assign_inv_sh: forall {CS: compspecs} {Espec: OracleKind} 
+  Delta e1 e2 P Q sh,
+@semax_aux CS Espec Delta P (Clight.Sassign e1 e2) Q ->
+  local (tc_environ Delta) && (allp_fun_id Delta && P) |-- 
+  !! (writable_share sh) &&
+  (|> ( (tc_lvalue Delta e1) &&  (tc_expr Delta (Ecast e2 (typeof e1))) 
+    &&
+             ((`(mapsto_ sh (typeof e1)) (eval_lvalue e1))))) ->
+  local (tc_environ Delta) && (allp_fun_id Delta && P) |-- 
+  (|> ( (tc_lvalue Delta e1) &&  (tc_expr Delta (Ecast e2 (typeof e1)))  &&
+             ((`(mapsto_ sh (typeof e1)) (eval_lvalue e1)) * (`(mapsto sh (typeof e1)) (eval_lvalue e1) (`force_val (`(sem_cast (typeof e2) (typeof e1)) (eval_expr e2))) -* RA_normal Q)))).
+Proof.
+  intros. revert dependent sh.
+  remember (Clight.Sassign e1 e2) as c eqn:?H.
+  induction H;try solve [inv H0].
+  + inv H0. intros sh'. intros.
+    eapply derives_trans. apply H0.
+  
+  reduce2derives.
+    apply later_derives; auto.
+    apply andp_derives; auto.
+    apply sepcon_derives; auto.
+    { assert (exists sh1, sepalg.join sh' sh1 sh).
+      { hnf in H. hnf in Hsh.
+        destruct Hsh as [E1 E2].
+        destruct H as [E3 E4]. hnf in E2. hnf in E4.
+        destruct E2 as [sh1 E2].
+        destruct E4 as [sh2 E4].
+        hnf in E2. hnf in E4.
+        destruct E2 as [E2 E5]. destruct E4 as [E4 E6].
+        Search Share.glb Share.bot. unfold sepalg.join.
+        unfold Share.Join_ba.V
+(** lub (Rsh , sh2) = sh',  lub (Rsh , sh3) = sh
+        gub (Rsh, sh2) = bot, lub (Rsh, sh3) = bot
+
+        
+        ? = glb (sh2, sh3)?
+        lub (lub (Rsh , sh2), ?) = lub (Rsh , sh3)
+        /\  glb (lub (Rsh , sh2), ?) = bot
+        
+        lub (sh', ?) = sh, gub (sh', ?) = bot
+
+      
+      
+      Goal: join (sh', ?) = sh *)
+
+
+        exists (Share.glb (Share.lub sh1 sh2) Share.Rsh).
+        hnf.
+        split.
+        (* - unfold nonempty_share. rewrite Share.distrib1.
+          hnf in E1. hnf in E3.
+          apply identityToken' in C. apply Share.identityToken in C.
+          apply lub_bot_e in C. destruct C.
+          apply Share.identityToken in H1. apply identityToken' in H1. contradiction.
+        - hnf.  hnf in E2. hnf in E4.
+          destruct E2 as [sh3 E2]. destruct E4 as [sh4 E4].
+          unfold sepalg.join in *. unfold Share.Join_ba in *.
+          exists (Share.lub sh3 sh4). destruct E2 as [E5 E6]. destruct E4 as [E7 E8]. *)
+          (* split. *)
+          + rewrite <- E6.
+            rewrite Share.glb_commute.
+            rewrite Share.distrib1.
+            admit.
+          + rewrite <- E5. rewrite <- E6.
+            rewrite Share.distrib2.
+            Search Share.glb. Share.lub.
+          
+          rewrite Share.lub_commute.
+            rewrite (Share.lub_commute sh1 sh2).
+            rewrite <- Share.distrib2. rewrite E2.
+            apply Share.lub_bot.
+          + rewrite <- E6. rewrite <- E8.
+            rewrite (Share.lub_commute (Share.Rsh) sh3).
+            rewrite Share.lub_assoc. rewrite <- (Share.lub_assoc Share.Rsh Share.Rsh).
+            rewrite Share.lub_idem. rewrite <- (Share.lub_assoc sh3).
+            rewrite (Share.lub_commute (sh3) (Share.Rsh)).
+            rewrite Share.lub_assoc. reflexivity.
+
+
+
+       }
+
+      Search sepalg.join sepalg.join_sub.
+      Search Share.glb sepalg.join.
+      
+      unfold sepalg.join_sub in H.
+      unfold sepalg.join in H.
+      unfold Share.Join_ba in H.
+      
+      
+      
+      
+      Search mapsto Share.t. }
+    apply wand_derives; auto.
+    apply derives_refl.
+  + subst c. specialize (IHsemax_aux eq_refl).
+    eapply derives_trans with (Q:= (andp (local (tc_environ Delta)) (andp (allp_fun_id Delta) P'))).
+    { repeat (apply andp_right;try solve_andp). auto. }
+    eapply derives_trans.
+    { apply andp_right with (P0:=local (tc_environ Delta)). solve_andp.
+      apply andp_right with (P0:=
+        allp_fun_id Delta). solve_andp. apply derives_refl. }
+    eapply derives_trans.
+    { apply andp_right. apply andp_left1. apply derives_refl.
+      apply andp_right. apply andp_left2. apply andp_left1. apply derives_refl.
+      apply andp_left2. apply andp_left2.
+      apply IHsemax_aux. }
+    reduceR. Intros sh. Exists sh.
+    apply andp_right.
+    { apply prop_right. auto. }
+    apply later_ENTAILL.
+    apply andp_ENTAILL; [reduceLL; apply ENTAIL_refl |].
+    apply sepcon_ENTAILL; [reduceLL; apply ENTAIL_refl |].
+    apply wand_ENTAILL; [reduceLL; apply ENTAIL_refl |].
+    auto.
+Qed. *)
+
 
 Fixpoint nobreak s :=
  match s with
@@ -358,73 +743,196 @@ Proof.
         apply add_andp in H11. rewrite H11. solve_andp.
 Qed.
 
-Lemma semax_aux_seq_inv_strong: forall CS Espec (Delta : tycontext) (P : environ -> mpred) 
-      (R : ret_assert) (h t : Clight.statement),
-    @semax CS Espec Delta P (Clight.Ssequence h  t)%C R ->
-    @semax CS Espec Delta P h
-         (overridePost
-            (EX Q : environ -> mpred,
-             !! semax_aux Delta Q t R && Q)%assert R).
+
+
+Lemma mapsto_wand_reduce: forall sh1 sh2 t p v Q,
+  sepalg.join_sub sh1 sh2 ->
+  mapsto sh2 t p v * (mapsto sh2 t p v  -* Q) 
+  |-- mapsto sh1 t p v  * (mapsto sh1 t p v  -* Q).
+Proof.
+  intros. destruct H.
+  rewrite <- (mapsto_share_join _ _ _ t p v H).
+  rewrite sepcon_assoc.
+  apply sepcon_derives;auto.
+  apply wand_frame_intro'.
+  rewrite <- !sepcon_assoc.
+  rewrite (mapsto_share_join _ _ _ t p v H).
+  apply wand_frame_elim.
+Qed.
+
+
+Lemma mapsto_at_share_join_W:
+  forall sh1 sh2 sh t v v1 v2,
+  sepalg.join sh1 sh2 sh ->
+  writable_share sh1 -> tc_val' t v1 ->
+  mapsto sh1 t v v1  * mapsto sh2 t v v2
+  |-- (mapsto sh t v v1).
 Proof.
   intros.
-  remember (Clight.Ssequence h t) as c eqn:?H.
-  induction H; try solve [inv H0].
-  + induction H; try solve [ inv H0 ].
-    * inv H0. clear IHsemax_aux1 IHsemax_aux2.
-      apply semax_aux_intro in H.
-      eapply semax_conseq; [.. | exact H].
-      - apply aux1_reduceR. apply aux2_reduceR. solve_andp.
-      - apply aux1_reduceR. apply aux2_reduceR.
-         destruct R; unfold overridePost, tycontext.RA_normal.
-        apply (exp_right Q).
-        apply andp_right; [apply prop_right |]; auto.
-        solve_andp.
-      - destruct R. unfold tycontext.RA_break, overridePost.
-        apply aux1_reduceR. apply aux2_reduceR. solve_andp.
-      - destruct R. unfold tycontext.RA_break, overridePost.
-        apply aux1_reduceR. apply aux2_reduceR. solve_andp.
-      - intro.  destruct R; unfold tycontext.RA_break, overridePost.
-        apply aux1_reduceR. apply aux2_reduceR. solve_andp.
-    * subst c.
-      pose proof IHsemax_aux eq_refl. clear IHsemax_aux.
-      eapply semax_conseq; [.. | exact H0]; auto.
-      - apply aux1_reduceR. apply aux2_reduceR.
-        eapply derives_trans;[|apply H]. solve_andp.
-      - unfold overridePost, tycontext.RA_normal.
-        destruct R' as [R'0 R'1 R'2 R'3] at 1; clear R'0 R'1 R'2 R'3.
-        destruct R as [R0 R1 R2 R3] at 1; clear R0 R1 R2 R3.
-        reduce2derives.
-        apply exp_derives.
-        intros Q.
-        normalize.
-        apply andp_right; [apply prop_right | auto].
-        eapply semax_aux_conseq; [.. | apply H6]; auto; try
-        apply derives_full_refl.
-      - destruct R, R'; auto. unfold tycontext.RA_break, overridePost in*.
-        apply aux1_reduceR. apply aux2_reduceR. admit.
-      - admit.
-      - admit.
-  + subst c.
-    pose proof IHsemax eq_refl. clear IHsemax.
-    apply semax_aux_intro.
-    eapply semax_aux_conseq; [.. | exact H0]; auto.
-    - unfold overridePost, tycontext.RA_normal.
-      destruct R' as [R'0 R'1 R'2 R'3] at 1; clear R'0 R'1 R'2 R'3.
-      destruct R as [R0 R1 R2 R3] at 1; clear R0 R1 R2 R3.
-      reduce2derives.
-      apply exp_derives.
-      intros Q.
-      normalize.
-      apply andp_right; [apply prop_right | auto].
-      eapply semax_aux_conseq; [.. | apply H6]; auto.
-      apply derives_full_refl.
-    - destruct R, R'; auto.
-    - destruct R, R'; auto.
-    - destruct R, R'; auto.
+  rewrite <- (mapsto_share_join _ _ _ t v v1 H).
+  apply sepcon_derives;auto.
+  pose proof join_writable_readable H H0.
+  unfold mapsto. destruct (access_mode t);auto.
+  destruct (type_is_volatile t);auto.
+  destruct v eqn:E;auto. if_tac;try tauto.
+  unfold tc_val'. apply andp_derives.
+  2:{ apply derives_refl. } apply prop_derives.
+  intros. destruct H4. split;auto.
+Qed.
+
+Lemma mapsto_wand_reduce_writable: forall sh1 sh2 t p v1 v2 Q,
+  writable_share sh1 ->
+  sepalg.join_sub sh1 sh2 ->
+  mapsto sh2 t p v1 * (mapsto sh2 t p v2  -* Q) 
+  |-- mapsto sh1 t p v1  * (mapsto sh1 t p v2  -* Q).
+Proof.
+  intros. destruct H0.
+  rewrite <- (mapsto_share_join _ _ _ t p v1 H0).
+  rewrite sepcon_assoc.
+  apply sepcon_derives;auto.
+  apply wand_frame_intro'.
+  rewrite <- !sepcon_assoc.
+  eapply derives_trans.
+  { apply sepcon_derives.
+    - assert_PROP (tc_val' t v2).
+      { sep_apply (mapsto_tc_val'). Intros. apply prop_right. auto. }
+      apply mapsto_at_share_join_W; eassumption.
+    - apply derives_refl.
+  }
+  apply wand_frame_elim.
+Qed.
+(* Lemma mapsto_wand_reduce_writable: forall sh1 sh2 t p v1 v2 Q,
+  writable_share sh1 ->
+  sepalg.join_sub sh1 sh2 -> tc_val' t v2 ->
+(` (mapsto_ sh2 (typeof e))) (eval_lvalue e) *
+((` (mapsto sh2 (typeof e))) (eval_lvalue e)
+   ((` force_val) ((` (sem_cast (typeof e0) (typeof e))) (eval_expr e0))) -*
+ Q1)
+ |-- 
+ (` (mapsto_ sh1 (typeof e))) (eval_lvalue e) *
+ ((` (mapsto sh1 (typeof e))) (eval_lvalue e)
+    ((` force_val) ((` (sem_cast (typeof e0) (typeof e))) (eval_expr e0))) -*
+  Q1). *)
+
+(* Lemma ws: writable_share Share.Rsh.
+Proof.
+  hnf. split.
+  - hnf.
+    intros C. apply identity_share_bot in C.
+    Search Share.glb Share.Lsh.
+  Search sepalg.identity Share.t. intros C. hnf in C.
+    Search Share.
+
+Search writable_share. *)
 
 
+Lemma share_split_eq: forall sh,
+  sh = Share.lub (fst (Share.split sh)) (snd (Share.split sh)).
+Proof.
+  intros. 
+  pose proof Share.split_together (fst (Share.split sh)) (snd (Share.split sh)) sh.
+  destruct (Share.split sh). rewrite <- H;auto.
+Qed.
+
+Lemma writable_share_join: forall sh1 sh2, writable_share sh1 ->
+  writable_share sh2 -> exists sh',
+  sepalg.join_sub sh' sh1 /\ sepalg.join_sub sh' sh2 /\ writable_share sh'.
+Proof.
+  intros.
+  destruct H as [E1 E2].
+  destruct H0 as [E4 E5].
+  destruct E2 as [sh1r [E2 E3]]. destruct E5 as [sh2r [E5 E6]].
+  exists (Share.lub Share.Rsh (Share.glb sh1r sh2r)).
+  repeat split.
+  + exists (Share.glb sh1r (Share.comp sh2r)).
+    repeat split.
+    * rewrite Share.glb_commute. rewrite Share.distrib1.
+      rewrite Share.glb_commute at 1.
+      rewrite <- (Share.glb_assoc Share.Rsh).
+      rewrite E2. rewrite Share.glb_commute. rewrite Share.glb_bot.
+      rewrite Share.lub_commute.
+      rewrite Share.lub_bot. rewrite Share.glb_assoc.
+      rewrite (Share.glb_commute _ sh2r).
+      rewrite <- (Share.glb_assoc _ sh2r).
+      rewrite (Share.glb_commute _ sh2r).
+      rewrite Share.comp2. rewrite (Share.glb_commute Share.bot). rewrite Share.glb_bot.
+      rewrite Share.glb_bot. reflexivity.
+    * rewrite Share.lub_assoc. rewrite <- E3.
+      f_equal. rewrite <- Share.distrib1. rewrite Share.comp1.
+      rewrite Share.glb_top. reflexivity.
+  + exists (Share.glb sh2r (Share.comp sh1r)).
+    repeat split.
+    * rewrite Share.glb_commute. rewrite Share.distrib1.
+      rewrite Share.glb_commute at 1.
+      rewrite <- (Share.glb_assoc Share.Rsh).
+      rewrite E5. rewrite Share.glb_commute. rewrite Share.glb_bot.
+      rewrite Share.lub_commute.
+      rewrite Share.lub_bot. rewrite Share.glb_assoc.
+      rewrite <- (Share.glb_assoc _ sh1r).
+      rewrite (Share.glb_commute _ sh1r).
+      rewrite Share.comp2. rewrite (Share.glb_commute Share.bot). rewrite Share.glb_bot.
+      rewrite Share.glb_bot. reflexivity.
+    * rewrite Share.lub_assoc. rewrite <- E6.
+      f_equal. rewrite (Share.glb_commute sh1r). rewrite <- Share.distrib1.
+      rewrite Share.comp1.
+      rewrite Share.glb_top. reflexivity.
+  + rewrite Share.distrib1.
+    rewrite glb_Lsh_Rsh. rewrite Share.lub_commute.
+    rewrite Share.lub_bot. hnf.
+    intros. apply identity_share_bot in H.
+    admit.
+  + exists (Share.glb sh1r sh2r).
+    split;auto. rewrite <- Share.glb_assoc. rewrite E2.
+    rewrite Share.glb_commute. rewrite Share.glb_bot. reflexivity.
+Admitted.
 
 
+(* Lemma writable_share_ews: forall sh, writable_share sh ->
+  sepalg.join_sub Ews sh.
+Proof.
+  intros. destruct H.
+  hnf in H. unfold Ews.
+  destruct H0 as [sh' H0].
+  hnf in H0. destruct H0. hnf.
+  unfold extern_retainer. exists (Share.lub (snd (Share.split Share.Lsh)) sh').
+  { split.
+    - rewrite share_distrib1'.
+      rewrite H0. rewrite glb_split.
+      rewrite Share.lub_bot. rewrite lub_bot'.
+      pose proof glb_Rsh_Lsh.
+      pose proof Share.split_together (fst (Share.split Share.Lsh)) (snd (Share.split Share.Lsh)) Share.Lsh.
+      assert (Share.split Share.Lsh =
+      (fst (Share.split Share.Lsh), snd (Share.split Share.Lsh)) ).
+      { destruct (Share.split Share.Lsh). reflexivity. }
+      specialize (H3 H4). clear H4.
+      pose proof Share.split_together (fst (Share.split sh')) (snd (Share.split sh')) sh'.
+      assert (Share.split sh' = (fst (Share.split sh'), snd (Share.split sh'))).
+      { destruct (Share.split sh'). reflexivity. }
+      specialize (H4 H5). clear H5.
+      rewrite <- H3 in H2. rewrite Share.distrib1 in H2.
+      apply lub_bot_e in H2. destruct H2.
+      rewrite <- H4 in H0. rewrite Share.distrib1 in H0.
+      apply lub_bot_e in H0. destruct H0.
+      rewrite H5. rewrite Share.glb_commute. rewrite 
+        Search Share.lub Share.bot.
+        Search Share.glb Share.lub.
+      }
+
+      rewrite <- H3 at 1.
+      2:{ destruct (Share.split Share.Lsh). reflexivity.  }
+      simpl.
+      
+      eq_refl.
+      Search Share.split Share.lub.
+      Search Share.glb Share.Rsh Share.Lsh.
+      Search Share.split Share.glb.
+
+
+    Search Share.glb Share.lub.  }
+  
+  exists Wsh.
+  split;auto.
+Qed. *)
 
 Theorem semax_aux_conj_rule: forall  CS Espec Delta P Q c Q1 Q2 ,
   @semax_aux CS Espec Delta P c (overridePost Q1 Q) ->
@@ -445,11 +953,264 @@ Proof.
       { eapply derives_trans;[|apply H]. solve_andp. }
       { eapply derives_trans;[|apply H0]. solve_andp. }
     }
-    { unfold RA_normal. apply ENTAIL_refl. }
-    { unfold RA_break. apply andp_left2. apply FF_left. }
-    { unfold RA_continue. apply andp_left2. apply FF_left. }
-    { intros. unfold RA_return. apply andp_left2. apply FF_left. }
+    { unfold RA_normal.  solve_andp. }
+    { unfold RA_break. repeat apply andp_left2. apply FF_left. }
+    { unfold RA_continue. repeat apply andp_left2. apply FF_left. }
+    { intros. unfold RA_return. repeat apply andp_left2. apply FF_left. }
     apply semax_aux_skip.
+  - intros. destruct Q as [Qn Qb Qc Qr]. unfold_der.
+    apply semax_aux_assign_inv in H0.
+    apply semax_aux_assign_inv in H. unfold_der.
+    assert (semax_aux Delta P (Clight.Sassign e e0)%C
+    {| RA_normal := Q1 && Q2;
+      RA_break := FF;
+      RA_continue := FF;
+      RA_return := FF |}).
+    { eapply semax_aux_conseq;
+       [..|apply semax_aux_assign with (P0:= Q1 && Q2)];
+        unfold normal_ret_assert;unfold_der;try (intros; solve_andp).
+      { pose proof andp_ENTAILL _ _ _ _ _ H0 H.
+        rewrite andp_dup in H1.
+        eapply derives_trans;[apply H1|]. clear H1.
+        Intros sh1. Intros sh2.
+        pose proof writable_share_join _ _ H1 H2.
+        destruct H3 as [sh' [E1 [E2 E3]]].
+        Exists sh'. apply andp_right.
+        { apply prop_right. auto. }
+        rewrite <- later_andp.
+        apply later_derives.
+        repeat apply andp_right; try solve_andp.
+        rewrite andp_assoc. apply andp_left2. unfold liftx. simpl. unfold lift.
+        unfold mapsto_. intros x.
+        eapply derives_trans.
+        { apply andp_derives.
+          { apply mapsto_wand_reduce_writable; try eassumption. }
+          apply andp_derives.
+          { apply+ derives_refl. }
+          { apply mapsto_wand_reduce_writable; try eassumption. }
+        } (* typecheck envrion? => tc_val t v2 *)
+        admit.
+      }
+    }
+    eapply semax_aux_noreturn_inv with (Post:={|
+      RA_normal := Q1 && Q2; RA_break := Qb; RA_continue := Qc; RA_return := FF
+    |});auto.
+    eapply semax_aux_nocontinue_inv with (Post:={|
+      RA_normal := Q1 && Q2; RA_break := Qb; RA_continue := FF; RA_return := FF
+    |});auto.
+    eapply semax_aux_nobreak_inv with (Post:={|
+      RA_normal := Q1 && Q2; RA_break := FF; RA_continue := FF; RA_return := FF
+    |});auto.
+  - intros. destruct Q as [Qn Qb Qc Qr]. unfold_der.
+    apply semax_aux_set_inv in H0.
+    apply semax_aux_set_inv in H. unfold_der.
+    assert (semax_aux Delta P (Clight.Sset i e)%C
+    {| RA_normal := Q1 && Q2;
+      RA_break := FF;
+      RA_continue := FF;
+      RA_return := FF |}).
+    { eapply semax_aux_conseq;
+      [..|apply semax_aux_set_ptr_compare_load_cast_load_backward with (P0:= Q1 && Q2)];
+        unfold normal_ret_assert;unfold_der;try (intros; solve_andp).
+      { pose proof andp_ENTAILL _ _ _ _ _ H0 H.
+        rewrite andp_dup in H1.
+        eapply derives_trans;[apply H1|]. clear H1.
+        rewrite !distrib_orp_andp. repeat apply orp_left.
+        + rewrite andp_comm. rewrite !distrib_orp_andp.
+          repeat apply orp_left.
+          * apply orp_right1. apply orp_right1.
+            apply orp_right1. rewrite <- later_andp.
+            apply later_derives. rewrite subst_andp.
+            solve_andp.
+          * eapply derives_trans;[|apply FF_left].
+            Intros cmp e1 e2 ty sh1 sh2.
+            admit.
+          * admit.
+          * admit.
+        + rewrite andp_comm. rewrite !distrib_orp_andp.
+          repeat apply orp_left.
+          * admit.
+          * apply orp_right1. apply orp_right1.
+            apply orp_right2. 
+            Intros cmpa e1a e2a tya sh1a sh2a.
+            Intros cmpb e1b e2b tyb sh1b sh2b.
+            rewrite <- later_andp.
+            Search TT sepcon.
+            apply later_derives. rewrite subst_andp.
+            solve_andp.
+            unfold tc_temp_id.
+            unfold typecheck_temp_id.
+            destruct ((temp_types Delta) ! i) eqn:E.
+            2:{  unfold tc_FF. }
+            unfold denote_tc_assert.
+            Search tc_temp_id.
+            Search tc_expr Ebinop.
+            unfold tc_temp_id.
+            unfold typecheck_temp_id.
+            unfold temp_types.
+          Search derives FF.
+            Search subst andp. solve_andp.
+        Search andp orp.
+
+
+
+        (* Intros sh1. Intros sh2.
+        pose proof writable_share_join _ _ H1 H2.
+        destruct H3 as [sh' [E1 [E2 E3]]].
+        Exists sh'. apply andp_right. *)
+        (* { apply prop_right. auto. } *)
+        
+        apply andp_right. try solve_andp.
+        apply later_derives.
+        repeat apply andp_right; try solve_andp.
+        rewrite andp_assoc. apply andp_left2. unfold liftx. simpl. unfold lift.
+        unfold mapsto_. intros x.
+        eapply derives_trans.
+        { apply andp_derives.
+          { apply mapsto_wand_reduce_writable; try eassumption. }
+          apply andp_derives.
+          { apply derives_refl. }
+          { apply mapsto_wand_reduce_writable; try eassumption. }
+        } (* typecheck envrion? => tc_val t v2 *)
+        admit.
+      }
+    }
+    
+  intros.
+    
+      { solve_andp. }
+          
+            Search force_val sem_cast.
+
+
+            + Search typecheck_environ. auto.
+            Check predicates_hered.app_pred.
+            Print juicy_mem.juicy_mem.
+            Check typecheck_environ.
+            Search tc_val force_val.
+            unfold tc_val'. intros. unfold force_val in *.
+            destruct (typeof e0), (typeof e);simpl in H3.
+            unfold sem_cast.
+            simpl.
+            
+            Search tc_val force_val.
+        }
+        
+        simpl.
+        
+        simpl.
+        unfold mapsto_.
+        rewrite andp_comm. intros r. simpl.
+          assert_PROP (tc_val' (typeof e) (eval_lvalue e r)).
+          { admit. }
+          eapply derives_trans.
+          { eapply andp_derives.
+            eapply andp_derives. { apply derives_refl. }
+            Search Ews.
+            Search juicy_mem.perm_of_sh.
+            apply mapsto_wand_reduce_writable.
+
+
+          }
+          eapply derives_andp. 
+          unfold mapsto_. simpl.
+          rewrite <-andp_assoc. apply andp_left1.
+          Search later andp.
+          Search andp.
+          Search allp_fun_id andp derives.
+
+           hnf. destruct H1 as [E1 E2]. destruct H2 as [E3 E4].
+          split.
+          - unfold nonempty_share. rewrite Share.distrib1.
+            hnf in E1. hnf in E3. intros C. Search sepalg.identity.
+            apply identityToken' in C. apply Share.identityToken in C.
+            apply lub_bot_e in C. destruct C.
+            apply Share.identityToken in H1. apply identityToken' in H1. contradiction.
+          - hnf.  hnf in E2. hnf in E4.
+            destruct E2 as [sh3 E2]. destruct E4 as [sh4 E4].
+            unfold sepalg.join in *. unfold Share.Join_ba in *.
+            exists (Share.lub sh3 sh4). destruct E2 as [E5 E6]. destruct E4 as [E7 E8].
+            split.
+            + rewrite Share.distrib1. rewrite E5. rewrite E7. apply Share.lub_bot.
+            + rewrite <- E6. rewrite <- E8.
+              rewrite (Share.lub_commute (Share.Rsh) sh3).
+              rewrite Share.lub_assoc. rewrite <- (Share.lub_assoc Share.Rsh Share.Rsh).
+              rewrite Share.lub_idem. rewrite <- (Share.lub_assoc sh3).
+              rewrite (Share.lub_commute (sh3) (Share.Rsh)).
+              rewrite Share.lub_assoc. reflexivity.
+         }
+         rewrite andp_assoc.
+         rewrite <- later_andp. rewrite andp_assoc.
+         eapply derives_trans.
+         { apply andp_right.
+          + rewrite <- andp_assoc. apply andp_left1.
+            rewrite <- andp_assoc. apply andp_left1. apply derives_refl.
+          + apply andp_left2. apply andp_left2. apply derives_refl. }
+        rewrite andp_assoc.
+        Search writable_share.
+        Search mapsto sepcon.
+        Search sepalg.joins Share.t.
+        Search sepalg.join Share.t.
+        Search sepalg.Join Share.t.
+        
+        
+        Search mapsto Share.t.
+         apply later_ENTAILL. apply andp_right;try solve_andp.
+         Search sepcon.
+         eapply andp_right.
+         Print andp_right.
+
+         (sepcon (liftx (mapsto_ (Share.lub sh1 sh2) (typeof e)) (eval_lvalue e))
+     (wand (liftx (mapsto (Share.lub sh1 sh2) (typeof e)) (eval_lvalue e) (liftx force_val (liftx (sem_cast (typeof e0) (typeof e)) (eval_expr e0))))
+        (andp Q1 Q2)))
+         apply andp_right.
+         
+         Search mapsto Share.t.
+Search mapsto mapsto_.
+         ((` (mapsto_ sh2 (typeof e))) (eval_lvalue e) *
+         ((` (mapsto sh2 (typeof e))) (eval_lvalue e) ((` force_val) ((` (sem_cast (typeof e0) (typeof e))) (eval_expr e0))) -* Q1))
+
+         Search sepalg.join ex.
+         Search sepalg.joins.
+         apply wand_ENTAILL.
+         Search "-*" andp. apply wand_ENTAIL.
+
+         Search later andp.
+          Search Share.lub sepalg.identity.
+            hnf.
+          simpl.
+        
+        }
+        Print writable_share.
+        Search Share.lub writable_share.
+        Search Share.t.
+        Check sepalg.join.
+        Search share.
+      }
+      { unfold normal_ret_assert. unfold RA_normal. solve_andp. }
+      { unfold normal_ret_assert. unfold RA_break. solve_andp. }
+      
+      2:{ unfold normal_ret_assert in HeqQ'. unfold_der. }
+      Search FF derives.
+
+  
+  
+  
+  admit.
+  - admit.
+  - admit.
+  - admit.
+  - intros. apply semax_aux_seq_inv in H0.
+    apply semax_aux_seq_inv in H.
+    destruct Q as [Qn Qb Qc Qr]. unfold_der.
+    destruct H0 as [R1 [? ?]].
+    destruct H as [R2 [? ?]].
+    specialize (IHc1 _ _ H _ H0).
+    eapply semax_aux_seq with (Q:= R1 && R2).
+    { unfold_der. auto. }
+    apply IHc2.
+    { eapply semax_aux_conseq;[..|apply H1];auto;unfold_der;try intros;solve_andp. }
+    { eapply semax_aux_conseq;[..|apply H2];auto;unfold_der;try intros;solve_andp. }
   - 
 
 Admitted.
